Proved.

src/riot/RIoT.Core.fst
@@ -67,7 +67,7 @@ let coerce_asn1_tlv_int32_of_type_to_asn1_int32 (x:asn1_TLV_int32_of_type SEQUEN
 
 unfold
 let deviceIDCSR_pre (x:deviceIDCSR_ingredients_t{deviceIDCRI_pre x}) (deviceIDCSR_len:UInt32.t) =
-  let l = coerce_asn1_tlv_int32_of_type_to_asn1_int32
+  let l = //coerce_asn1_tlv_int32_of_type_to_asn1_int32
     (len_of_deviceIDCRI
       x.deviceIDCSR_version x.deviceIDCSR_s_common x.deviceIDCSR_s_org
       x.deviceIDCSR_s_country) in
@@ -77,7 +77,7 @@ let deviceIDCSR_pre (x:deviceIDCSR_ingredients_t{deviceIDCRI_pre x}) (deviceIDCS
 
 unfold
 let aliasKeyCRT_pre (x:aliasKeyCRT_ingredients_t) (aliasKeyCRT_len:UInt32.t) =
-  let l = coerce_asn1_tlv_int32_of_type_to_asn1_int32
+  let l = //coerce_asn1_tlv_int32_of_type_to_asn1_int32
     (len_of_aliasKeyTBS
       x.aliasKeyCrt_serialNumber x.aliasKeyCrt_i_common x.aliasKeyCrt_i_org x.aliasKeyCrt_i_country
       x.aliasKeyCrt_s_common x.aliasKeyCrt_s_org x.aliasKeyCrt_s_country
@@ -91,9 +91,9 @@ let riot_pre
 (* Common Inputs *)
   (cdi : B.lbuffer byte_sec 32)
   (fwid: B.lbuffer byte_sec 32)
-  (deviceID_label_len: size_t)
+  (deviceID_label_len: UInt32.t)
   (deviceID_label: B.lbuffer byte_sec (v deviceID_label_len))
-  (aliasKey_label_len: size_t)
+  (aliasKey_label_len: UInt32.t)
   (aliasKey_label: B.lbuffer byte_sec (v aliasKey_label_len))
 (* DeviceID CSR Inputs*)
   (deviceIDCSR_ingredients:deviceIDCSR_ingredients_t)
@@ -103,10 +103,10 @@ let riot_pre
   (aliasKey_pub: B.lbuffer byte_pub 32)
   (aliasKey_priv: B.lbuffer uint8 32)
 (* DeviceID CSR Outputs *)
-  (deviceIDCSR_len: size_t)
+  (deviceIDCSR_len: UInt32.t)
   (deviceIDCSR_buf: B.lbuffer byte_pub (v deviceIDCSR_len))
 (* AliasKey Crt Outputs *)
-  (aliasKeyCRT_len: size_t)
+  (aliasKeyCRT_len: UInt32.t)
   (aliasKeyCRT_buf: B.lbuffer byte_pub (v aliasKeyCRT_len))
 : Type0
 =   B.(all_live h [buf cdi;
@@ -145,10 +145,9 @@ let aliasKey_post
     (B.as_seq h1 aliasKey_priv <: lbytes_sec 32)) == derive_AliasKey_spec
                                                        (B.as_seq h0 cdi)
                                                        (B.as_seq h0 fwid)
-                                                       aliasKey_label_len
+                                                       (aliasKey_label_len)
                                                        (B.as_seq h0 aliasKey_label)
 
-#push-options "--z3rlimit 100"
 unfold
 let deviceIDCSR_post
   (cdi:B.lbuffer byte_sec 32)
@@ -176,16 +175,15 @@ let deviceIDCSR_post
         deviceIDCSR_ingredients.deviceIDCSR_version deviceIDCSR_ingredients.deviceIDCSR_s_common
         deviceIDCSR_ingredients.deviceIDCSR_s_org deviceIDCSR_ingredients.deviceIDCSR_s_country) in
 
-    let (* Prf *) _ = lemma_serialize_deviceIDCRI_size_exact deviceIDCRI in  //AR: TODO: This takes long time
+    let (* Prf *) _ = lemma_serialize_deviceIDCRI_size_exact deviceIDCRI in
     let deviceIDCSR: deviceIDCSR_t deviceIDCRI_len = sign_and_finalize_deviceIDCSR_spec
                                                                 (deviceID_priv_seq)
                                                                 (deviceIDCRI_len)
                                                                 (deviceIDCRI_seq) in
     B.as_seq h1 deviceIDCSR_buf == serialize_deviceIDCSR deviceIDCRI_len `serialize` deviceIDCSR
-#pop-options
 
-unfold noextract
-let coerce_asn1_int32_to_size_t (x:asn1_int32) : size_t = x
+// unfold noextract
+// let coerce_asn1_int32_to_size_t (x:asn1_int32) : UInt32.t = x
 
 #push-options "--z3rlimit 100"
 unfold
@@ -205,7 +203,7 @@ let aliasKeyCRT_post
                                                  (deviceID_label_len)
                                                  (B.as_seq h0 deviceID_label) in
     let aliasKeyCrt_keyID_seq: lbytes_pub 20 =
-     derive_authKeyID_from_cdi_spec (B.as_seq h0 cdi) (deviceID_label_len) (B.as_seq h0 deviceID_label) in
+      derive_authKeyID_spec (classify_public_bytes deviceID_pub_seq) in
     let aliasKeyTBS = create_aliasKeyTBS_spec
       aliasKeyCRT_ingredients.aliasKeyCrt_version
       aliasKeyCRT_ingredients.aliasKeyCrt_serialNumber
@@ -224,7 +222,7 @@ let aliasKeyCRT_post
       deviceID_pub_seq
       (B.as_seq h1 aliasKey_pub) in
      let aliasKeyTBS_seq = serialize_aliasKeyTBS `serialize` aliasKeyTBS in
-     let aliasKeyTBS_len = coerce_asn1_tlv_int32_of_type_to_asn1_int32
+     let aliasKeyTBS_len = //coerce_asn1_tlv_int32_of_type_to_asn1_int32
        (len_of_aliasKeyTBS
          aliasKeyCRT_ingredients.aliasKeyCrt_serialNumber
          aliasKeyCRT_ingredients.aliasKeyCrt_i_common
@@ -241,15 +239,16 @@ let aliasKeyCRT_post
                                                                 (aliasKeyTBS_len)
                                                                 (aliasKeyTBS_seq) in
      B.as_seq h1 aliasKeyCRT_buf == serialize_aliasKeyCRT aliasKeyTBS_len `serialize` aliasKeyCRT
+#pop-options
 
 unfold
 let riot_post
 (* Common Inputs *)
   (cdi : B.lbuffer byte_sec 32)
   (fwid: B.lbuffer byte_sec 32)
-  (deviceID_label_len: size_t)
+  (deviceID_label_len: UInt32.t)
   (deviceID_label: B.lbuffer byte_sec (v deviceID_label_len))
-  (aliasKey_label_len: size_t)
+  (aliasKey_label_len: UInt32.t)
   (aliasKey_label: B.lbuffer byte_sec (v aliasKey_label_len))
 (* DeviceID CSR Inputs*)
   (deviceIDCSR_ingredients:deviceIDCSR_ingredients_t)
@@ -276,315 +275,28 @@ let riot_post
     B.(modifies (loc_buffer aliasKey_pub    `loc_union`
                  loc_buffer aliasKey_priv   `loc_union`
                  loc_buffer deviceIDCSR_buf `loc_union`
-                 loc_buffer aliasKeyCRT_buf
-                 ) h0 h1) /\
+                 loc_buffer aliasKeyCRT_buf) h0 h1) /\
 
     aliasKey_post cdi fwid aliasKey_label_len aliasKey_label aliasKey_pub aliasKey_priv h0 h1 /\
 
-    // deviceIDCSR_post cdi deviceID_label_len deviceID_label
-    //   deviceIDCSR_ingredients deviceIDCSR_len deviceIDCSR_buf h0 h1 /\
+    deviceIDCSR_post cdi deviceID_label_len deviceID_label
+      deviceIDCSR_ingredients deviceIDCSR_len deviceIDCSR_buf h0 h1 /\
 
-    // aliasKeyCRT_post cdi fwid deviceID_label_len deviceID_label
-    //   aliasKeyCRT_ingredients aliasKeyCRT_len aliasKeyCRT_buf aliasKey_pub h0 h1 /\
+    aliasKeyCRT_post cdi fwid deviceID_label_len deviceID_label
+      aliasKeyCRT_ingredients aliasKeyCRT_len aliasKeyCRT_buf aliasKey_pub h0 h1 /\
 True
-
-let () = ()
-// let f ()
-// : HST.St unit
-// = let h0 = HST.get () in
-//   HST.push_frame ();
-//   HST.pop_frame ();
-//   let h1 = HST.get () in
-//   assert (HST.equal_domains h0 h1)
 
 module U32 = FStar.UInt32
 module U8 = FStar.UInt8
 #reset-options
-
-(* NOTE: This lemma is verified and copied from `RIoT.Core.Lemmas` for convenience. *)
-#set-options "--lax"
-let lemma_help
-  (pub_t sec_t: Type0)
-  (h0 hs0 hsf hf: HS.mem)
-  (in1: B.buffer sec_t) (in2: B.buffer sec_t) (in3: B.buffer sec_t) (in4: B.buffer sec_t)
-  (out1: B.buffer pub_t) (out2: B.buffer sec_t) (out3: B.buffer pub_t) (out4: B.buffer pub_t)
-  (hs1 hs2 hs3 hs4 hs5 hs6 hs7 hs8 hs9 hs10 hs11 hs12 hs13 hs14: HS.mem)
-  (_bl1: UInt32.t) (_b1: B.lbuffer pub_t (U32.v _bl1)) (_bv1: pub_t)
-  (_bl2: UInt32.t) (_b2: B.lbuffer sec_t (U32.v _bl2)) (_bv2: sec_t)
-  (_bl3: UInt32.t) (_b3: B.lbuffer sec_t (U32.v _bl3)) (_bv3: sec_t)
-  (_bl4: UInt32.t) (_b4: B.lbuffer pub_t (U32.v _bl4)) (_bv4: pub_t)
-  (_bl5: UInt32.t) (_b5: B.lbuffer pub_t (U32.v _bl5)) (_bv5: pub_t)
-  (_bl6: UInt32.t) (_b6: B.lbuffer pub_t (U32.v _bl6)) (_bv6: pub_t)
-: Lemma
-  (requires
-            B.all_live h0 [B.buf in1; B.buf in2; B.buf in3; B.buf in4;
-                           B.buf out1; B.buf out2; B.buf out3; B.buf out4] /\
-            B.all_disjoint [B.loc_buffer in1; B.loc_buffer in2; B.loc_buffer in3; B.loc_buffer in4;
-                            B.loc_buffer out1; B.loc_buffer out2; B.loc_buffer out3; B.loc_buffer out4] /\
-            HS.fresh_frame h0 hs0 /\ HS.get_tip hs0 == HS.get_tip hsf /\ HS.popped hsf hf /\
-            B.alloc_post_mem_common _b1 hs0 hs1 (Seq.create (UInt32.v _bl1) _bv1) /\ B.frameOf _b1 == HS.get_tip hs0 /\
-            B.alloc_post_mem_common _b2 hs1 hs2 (Seq.create (UInt32.v _bl2) _bv2) /\ B.frameOf _b2 == HS.get_tip hs1 /\
-            B.alloc_post_mem_common _b3 hs2 hs3 (Seq.create (UInt32.v _bl3) _bv3) /\ B.frameOf _b3 == HS.get_tip hs2 /\
-            B.alloc_post_mem_common _b4 hs3 hs4 (Seq.create (UInt32.v _bl4) _bv4) /\ B.frameOf _b4 == HS.get_tip hs3 /\
-
-            (* Derive DeviceID *)
-            B.modifies (B.loc_buffer _b1 `B.loc_union` B.loc_buffer _b2) hs4 hs5 /\
-
-            (* Derive AliasKey *)
-            B.modifies (B.loc_buffer out1 `B.loc_union` B.loc_buffer out2) hs5 hs6 /\
-
-            (* Classify DeviceID Public Key *)
-            B.modifies (B.loc_buffer _b3) hs6 hs7 /\
-
-            (* Derive AliasCRT_AuthKeyID *)
-            B.modifies (B.loc_buffer _b4) hs7 hs8 /\
-
-            (* Allocate `deviceIDCRI_buf` *)
-            B.alloc_post_mem_common _b5 hs8 hs9 (Seq.create (UInt32.v _bl5) _bv5) /\ B.frameOf _b5 == HS.get_tip hs8 /\
-
-            (* Write `deviceIDCRI_buf` *)
-            B.modifies (B.loc_buffer _b5) hs9 hs10 /\
-
-            (* Write `deviceIDCSR_buf` *)
-            B.modifies (B.loc_buffer out3) hs10 hs11 /\
-
-            (* Allocate `aliasKeyTBS_buf` *)
-            B.alloc_post_mem_common _b6 hs11 hs12 (Seq.create (UInt32.v _bl6) _bv6) /\ B.frameOf _b6 == HS.get_tip hs11 /\
-
-            (* Write `aliasKeyTBS_buf` *)
-            B.modifies (B.loc_buffer _b6) hs12 hs13 /\
-
-            (* Write `aliasKeyCRT_buf` *)
-            B.modifies (B.loc_buffer out4) hs13 hs14 /\
-
-            hs14 == hsf
-            )
-  (ensures
-    B.modifies (B.loc_buffer out1 `B.loc_union`
-                B.loc_buffer out2 `B.loc_union`
-                B.loc_buffer out3 `B.loc_union`
-                B.loc_buffer out4) h0 hf /\
-
-    B.as_seq hs4  in1  == B.as_seq h0 in1 /\ // cdi
-    B.as_seq hs4  in3  == B.as_seq h0 in3 /\ // lbl device
-
-    B.as_seq hs5  in1  == B.as_seq h0 in1 /\ // cdi
-    B.as_seq hs5  in2  == B.as_seq h0 in2 /\ // fwid
-    B.as_seq hs5  in4  == B.as_seq h0 in4 /\ // lbl alias
-
-    B.as_seq hs6  out1 == B.as_seq hf out1 /\
-    B.as_seq hs6  out2 == B.as_seq hf out2 /\
-    B.as_seq hs11 out3 == B.as_seq hf out3 /\
-    B.as_seq hs14 out4 == B.as_seq hf out4 /\
-    True
-  )
-=
-  B.modifies_trans B.loc_none h0 hs0 B.loc_none hs1;
-  B.modifies_trans B.loc_none h0 hs1 B.loc_none hs2;
-  B.modifies_trans B.loc_none h0 hs2 B.loc_none hs3;
-  B.modifies_trans B.loc_none h0 hs3 B.loc_none hs4;
-
-  B.modifies_buffer_elim in1 B.loc_none h0 hs4;
-  B.modifies_buffer_elim in3 B.loc_none h0 hs4;
-
-(* hs4 --> hs5 *)
-  B.modifies_trans B.loc_none h0 hs4 (
-    B.loc_buffer _b1 `B.loc_union`
-    B.loc_buffer _b2
-  ) hs5;
-  B.modifies_buffer_elim in1 (B.loc_buffer out1 `B.loc_union` B.loc_buffer out2) h0 hs5;
-  B.modifies_buffer_elim in2 (B.loc_buffer out1 `B.loc_union` B.loc_buffer out2) h0 hs5;
-  B.modifies_buffer_elim in4 (B.loc_buffer out1 `B.loc_union` B.loc_buffer out2) h0 hs5;
-
-(* hs5 --> hs6 *)
-  B.modifies_trans (
-    B.loc_buffer _b1 `B.loc_union`
-    B.loc_buffer _b2
-  ) h0 hs5 (
-    B.loc_buffer out1 `B.loc_union`
-    B.loc_buffer out2
-  ) hs6;
-  B.modifies_buffer_elim _b1 (B.loc_buffer out1 `B.loc_union` B.loc_buffer out2) hs5 hs6;
-  B.modifies_buffer_elim _b2 (B.loc_buffer out1 `B.loc_union` B.loc_buffer out2) hs5 hs6;
-
-(* hs6 --> hs7 *)
-  B.modifies_trans (
-    B.loc_buffer _b1 `B.loc_union`
-    B.loc_buffer _b2 `B.loc_union`
-    B.loc_buffer out1  `B.loc_union`
-    B.loc_buffer out2
-  ) h0 hs6 (
-    B.loc_buffer _b3
-  ) hs7;
-  B.modifies_buffer_elim _b1 (B.loc_buffer _b3) hs6 hs7;
-  B.modifies_buffer_elim _b2 (B.loc_buffer _b3) hs6 hs7;
-  B.modifies_buffer_elim out1  (B.loc_buffer _b3) hs6 hs7;
-  B.modifies_buffer_elim out2  (B.loc_buffer _b3) hs6 hs7;
-
-(* hs7 --> hs8 *)
-  B.modifies_trans (
-    B.loc_buffer _b1 `B.loc_union`
-    B.loc_buffer _b2 `B.loc_union`
-    B.loc_buffer out1  `B.loc_union`
-    B.loc_buffer out2  `B.loc_union`
-    B.loc_buffer _b3
-  ) h0 hs7 (
-    B.loc_buffer _b4
-  ) hs8;
-  B.modifies_buffer_elim _b1 (B.loc_buffer _b4) hs7 hs8;
-  B.modifies_buffer_elim _b2 (B.loc_buffer _b4) hs7 hs8;
-  B.modifies_buffer_elim out1  (B.loc_buffer _b4) hs7 hs8;
-  B.modifies_buffer_elim out2  (B.loc_buffer _b4) hs7 hs8;
-  B.modifies_buffer_elim _b3 (B.loc_buffer _b4) hs7 hs8;
-
-(* hs8 --> hs9 *)
-  B.modifies_trans (
-    B.loc_buffer _b1 `B.loc_union`
-    B.loc_buffer _b2 `B.loc_union`
-    B.loc_buffer out1  `B.loc_union`
-    B.loc_buffer out2  `B.loc_union`
-    B.loc_buffer _b3 `B.loc_union`
-    B.loc_buffer _b4
-  ) h0 hs8 B.loc_none hs9;
-  B.modifies_buffer_elim _b1 B.loc_none hs8 hs9;
-  B.modifies_buffer_elim _b2 B.loc_none hs8 hs9;
-  B.modifies_buffer_elim out1  B.loc_none hs8 hs9;
-  B.modifies_buffer_elim out2  B.loc_none hs8 hs9;
-  B.modifies_buffer_elim _b3 B.loc_none hs8 hs9;
-  B.modifies_buffer_elim _b4 B.loc_none hs8 hs9;
-
-(* hs9 --> hs10 *)
-  B.modifies_trans (
-    B.loc_buffer _b1 `B.loc_union`
-    B.loc_buffer _b2 `B.loc_union`
-    B.loc_buffer out1  `B.loc_union`
-    B.loc_buffer out2  `B.loc_union`
-    B.loc_buffer _b3 `B.loc_union`
-    B.loc_buffer _b4
-  ) h0 hs9 (
-    B.loc_buffer _b5
-  ) hs10;
-  B.modifies_buffer_elim _b1 (B.loc_buffer _b5) hs9 hs10;
-  B.modifies_buffer_elim _b2 (B.loc_buffer _b5) hs9 hs10;
-  B.modifies_buffer_elim out1  (B.loc_buffer _b5) hs9 hs10;
-  B.modifies_buffer_elim out2  (B.loc_buffer _b5) hs9 hs10;
-  B.modifies_buffer_elim _b3 (B.loc_buffer _b5) hs9 hs10;
-  B.modifies_buffer_elim _b4 (B.loc_buffer _b5) hs9 hs10;
-
-
-(* hs10 --> hs11 *)
-  B.modifies_trans (
-    B.loc_buffer _b1 `B.loc_union`
-    B.loc_buffer _b2 `B.loc_union`
-    B.loc_buffer out1  `B.loc_union`
-    B.loc_buffer out2  `B.loc_union`
-    B.loc_buffer _b3 `B.loc_union`
-    B.loc_buffer _b4 `B.loc_union`
-    B.loc_buffer _b5
-  ) h0 hs10 (
-    B.loc_buffer out3
-  ) hs11;
-  B.modifies_buffer_elim _b1 (B.loc_buffer out3) hs10 hs11;
-  B.modifies_buffer_elim _b2 (B.loc_buffer out3) hs10 hs11;
-  B.modifies_buffer_elim out1  (B.loc_buffer out3) hs10 hs11;
-  B.modifies_buffer_elim out2  (B.loc_buffer out3) hs10 hs11;
-  B.modifies_buffer_elim _b3 (B.loc_buffer out3) hs10 hs11;
-  B.modifies_buffer_elim _b4 (B.loc_buffer out3) hs10 hs11;
-  B.modifies_buffer_elim _b5 (B.loc_buffer out3) hs10 hs11;
-
-(* hs11 --> hs12 *)
-  B.modifies_trans (
-    B.loc_buffer _b1 `B.loc_union`
-    B.loc_buffer _b2 `B.loc_union`
-    B.loc_buffer out1  `B.loc_union`
-    B.loc_buffer out2  `B.loc_union`
-    B.loc_buffer _b3 `B.loc_union`
-    B.loc_buffer _b4 `B.loc_union`
-    B.loc_buffer _b5 `B.loc_union`
-    B.loc_buffer out3
-  ) h0 hs11 B.loc_none hs12;
-  B.modifies_buffer_elim _b1 B.loc_none hs11 hs12;
-  B.modifies_buffer_elim _b2 B.loc_none hs11 hs12;
-  B.modifies_buffer_elim out1  B.loc_none hs11 hs12;
-  B.modifies_buffer_elim out2  B.loc_none hs11 hs12;
-  B.modifies_buffer_elim _b3 B.loc_none hs11 hs12;
-  B.modifies_buffer_elim _b4 B.loc_none hs11 hs12;
-  B.modifies_buffer_elim _b5 B.loc_none hs11 hs12;
-  B.modifies_buffer_elim out3  B.loc_none hs11 hs12;
-
-(* hs12 --> hs13 *)
-  B.modifies_trans (
-    B.loc_buffer _b1 `B.loc_union`
-    B.loc_buffer _b2 `B.loc_union`
-    B.loc_buffer out1  `B.loc_union`
-    B.loc_buffer out2  `B.loc_union`
-    B.loc_buffer _b3 `B.loc_union`
-    B.loc_buffer _b4 `B.loc_union`
-    B.loc_buffer _b5 `B.loc_union`
-    B.loc_buffer out3
-  ) h0 hs12 (
-    B.loc_buffer _b6
-  ) hs13;
-  B.modifies_buffer_elim _b1 (B.loc_buffer _b6) hs12 hs13;
-  B.modifies_buffer_elim _b2 (B.loc_buffer _b6) hs12 hs13;
-  B.modifies_buffer_elim out1  (B.loc_buffer _b6) hs12 hs13;
-  B.modifies_buffer_elim out2  (B.loc_buffer _b6) hs12 hs13;
-  B.modifies_buffer_elim _b3 (B.loc_buffer _b6) hs12 hs13;
-  B.modifies_buffer_elim _b4 (B.loc_buffer _b6) hs12 hs13;
-  B.modifies_buffer_elim _b5 (B.loc_buffer _b6) hs12 hs13;
-  B.modifies_buffer_elim out3  (B.loc_buffer _b6) hs12 hs13;
-
-(* hs13 --> hs14 *)
-  B.modifies_trans (
-    B.loc_buffer _b1 `B.loc_union`
-    B.loc_buffer _b2 `B.loc_union`
-    B.loc_buffer out1  `B.loc_union`
-    B.loc_buffer out2  `B.loc_union`
-    B.loc_buffer _b3 `B.loc_union`
-    B.loc_buffer _b4 `B.loc_union`
-    B.loc_buffer _b5 `B.loc_union`
-    B.loc_buffer out3  `B.loc_union`
-    B.loc_buffer _b6
-  ) h0 hs13 (
-    B.loc_buffer out4
-  ) hs14;
-  B.modifies_buffer_elim _b1 (B.loc_buffer out4) hs13 hs14;
-  B.modifies_buffer_elim _b2 (B.loc_buffer out4) hs13 hs14;
-  B.modifies_buffer_elim out1  (B.loc_buffer out4) hs13 hs14;
-  B.modifies_buffer_elim out2  (B.loc_buffer out4) hs13 hs14;
-  B.modifies_buffer_elim _b3 (B.loc_buffer out4) hs13 hs14;
-  B.modifies_buffer_elim _b4 (B.loc_buffer out4) hs13 hs14;
-  B.modifies_buffer_elim _b5 (B.loc_buffer out4) hs13 hs14;
-  B.modifies_buffer_elim out3  (B.loc_buffer out4) hs13 hs14;
-  B.modifies_buffer_elim _b6 (B.loc_buffer out4) hs13 hs14;
-
-(* FIXME: This can be proved with 256-512 z3rlimits *)
-  assume (B.modifies ((B.loc_all_regions_from false (HS.get_tip hs0)) `B.loc_union`
-                      (B.loc_buffer out1 `B.loc_union`
-                       B.loc_buffer out2 `B.loc_union`
-                       B.loc_buffer out3 `B.loc_union`
-                       B.loc_buffer out4)) hs0 hsf);
-
-  B.modifies_fresh_frame_popped h0 hs0 (
-    B.loc_buffer out1 `B.loc_union`
-    B.loc_buffer out2 `B.loc_union`
-    B.loc_buffer out3 `B.loc_union`
-    B.loc_buffer out4
-  ) hsf hf;
-
-()
-
-let () = ()
-
-#restart-solver
-#set-options "--z3rlimit 50 --fuel 0 --ifuel 0"
+#set-options "--z3rlimit 400 --fuel 0 --ifuel 0"
 let riot
 (* Common Inputs *)
   (cdi : B.lbuffer byte_sec 32)
   (fwid: B.lbuffer byte_sec 32)
-  (deviceID_label_len: size_t)
+  (deviceID_label_len: UInt32.t)
   (deviceID_label: B.lbuffer byte_sec (v deviceID_label_len))
-  (aliasKey_label_len: size_t)
+  (aliasKey_label_len: UInt32.t)
   (aliasKey_label: B.lbuffer byte_sec (v aliasKey_label_len))
 (* DeviceID CSR Inputs*)
   (deviceIDCSR_ingredients:deviceIDCSR_ingredients_t)
@@ -594,10 +306,10 @@ let riot
   (aliasKey_pub: B.lbuffer byte_pub 32)
   (aliasKey_priv: B.lbuffer uint8 32)
 (* DeviceID CSR Outputs *)
-  (deviceIDCSR_len: size_t)
+  (deviceIDCSR_len: UInt32.t)
   (deviceIDCSR_buf: B.lbuffer byte_pub (v deviceIDCSR_len))
 (* AliasKey Crt Outputs *)
-  (aliasKeyCRT_len: size_t)
+  (aliasKeyCRT_len: UInt32.t)
   (aliasKeyCRT_buf: B.lbuffer byte_pub (v aliasKeyCRT_len))
 : HST.Stack unit
   (requires fun h ->
@@ -627,148 +339,88 @@ let riot
   HST.push_frame ();
   (**) let hs0 = HST.get () in
   (**) B.fresh_frame_modifies h0 hs0;
-  // (**) B.modifies_buffer_elim cdi B.loc_none h0 hs0;
-
 
 (* Derive DeviceID *)
   let deviceID_pub : B.lbuffer byte_pub 32 = B.alloca 0x00uy    32ul in
   let hs1 = HST.get () in
   let deviceID_priv: B.lbuffer byte_sec 32 = B.alloca (u8 0x00) 32ul in
   let hs2 = HST.get () in
-  let deviceID_pub_sec: B.lbuffer byte_sec 32 = B.alloca (u8 0x00) 32ul in
+  let authKeyID: B.lbuffer byte_pub 20 = B.alloca 0x00uy 20ul in
   let hs3 = HST.get () in
-  let aliasKeyCrt_keyID: B.lbuffer byte_pub 20 = B.alloca 0x00uy 20ul in
-  let hs4 = HST.get () in
 
-  assume (
-    B.(all_live hs4 [buf deviceID_pub;
-                     buf deviceID_priv;
-                     buf cdi;
-                     buf deviceID_label]) /\
-    B.(all_disjoint [loc_buffer deviceID_pub;
-                     loc_buffer deviceID_priv;
-                     loc_buffer cdi;
-                     loc_buffer deviceID_label])
-  );
-  printf "Deriving DeviceID\n" done;
-  derive_DeviceID
-    (* pub *) deviceID_pub
-    (* priv*) deviceID_priv
-    (* cdi *) cdi
-    (* lbl *) deviceID_label_len
-              deviceID_label;
-(* hs5 *) let hs5 = HST.get () in
+  let _h_step1_pre = HST.get () in
+  (**) B.modifies_buffer_elim cdi  B.loc_none h0 hs3;
+  (**) B.modifies_buffer_elim fwid B.loc_none h0 hs3;
+  (**) B.modifies_buffer_elim deviceID_label B.loc_none h0 hs3;
+  (**) B.modifies_buffer_elim deviceID_label B.loc_none h0 hs3;
+  riot_core_step1
+    (cdi) (fwid)
+    (deviceID_label_len) (deviceID_label)
+    (aliasKey_label_len) (aliasKey_label)
+    (deviceID_pub) (deviceID_priv)
+    (aliasKey_pub) (aliasKey_priv)
+    (authKeyID);
+  let _h_step1_post = HST.get () in
+  (**) let hs4 = HST.get () in
 
-  assume (
-    B.(all_live hs5 [buf aliasKey_pub;
-                     buf aliasKey_priv;
-                     buf cdi;
-                     buf fwid;
-                     buf aliasKey_label]) /\
-    B.(all_disjoint [loc_buffer aliasKey_pub;
-                     loc_buffer aliasKey_priv;
-                     loc_buffer cdi;
-                     loc_buffer fwid;
-                     loc_buffer aliasKey_label])
-  );
-  printf "Deriving AliasKey\n" done;
-  derive_AliasKey
-    (* pub *) aliasKey_pub
-    (* priv*) aliasKey_priv
-    (* cdi *) cdi
-    (* fwid*) fwid
-    (* lbl *) aliasKey_label_len
-              aliasKey_label;
-(* hs6 *) let hs6 = HST.get () in
+  assert (aliasKey_post cdi fwid aliasKey_label_len aliasKey_label aliasKey_pub aliasKey_priv h0 _h_step1_post);
 
-  assert ( aliasKey_post cdi fwid aliasKey_label_len aliasKey_label aliasKey_pub aliasKey_priv hs5 hs6 );
-  // assume ( B.as_seq hs5 cdi == B.as_seq h0 cdi /\
-  //          B.as_seq hs5 fwid == B.as_seq h0 fwid /\
-  //          B.as_seq hs5 aliasKey_label == B.as_seq h0 aliasKey_label);
-  // assert ( aliasKey_post cdi fwid aliasKey_label_len aliasKey_label aliasKey_pub aliasKey_priv h0 hs6 );
+  (**) B.modifies_trans B.loc_none h0 hs3 (
+    B.loc_buffer deviceID_pub  `B.loc_union`
+    B.loc_buffer deviceID_priv `B.loc_union`
+    B.loc_buffer aliasKey_pub  `B.loc_union`
+    B.loc_buffer aliasKey_priv `B.loc_union`
+    B.loc_buffer authKeyID
+  ) hs4;
 
-  assume (
-    B.live hs6 deviceID_pub /\ B.live hs6 deviceID_pub_sec /\
-    B.disjoint deviceID_pub deviceID_pub_sec
-  );
-  classify_public_buffer 32ul deviceID_pub deviceID_pub_sec;
-(* hs7 *) let hs7 = HST.get () in
+  let _h_step2_pre = _h_step1_post in
 
-  assume (
-    B.live hs7 aliasKeyCrt_keyID /\ B.live hs7 deviceID_pub_sec /\
-    B.disjoint aliasKeyCrt_keyID deviceID_pub_sec
-  );
-  derive_authKeyID
-    aliasKeyCrt_keyID
-    deviceID_pub_sec;
-(* hs8 *) let hs8 = HST.get () in
-
-(* Create DeviceIDCRI *)
-   let deviceIDCRI_len: asn1_TLV_int32_of_type SEQUENCE = len_of_deviceIDCRI
-                                                            deviceIDCSR_ingredients.deviceIDCSR_version
-                                                            deviceIDCSR_ingredients.deviceIDCSR_s_common
-                                                            deviceIDCSR_ingredients.deviceIDCSR_s_org
-                                                            deviceIDCSR_ingredients.deviceIDCSR_s_country in
-   let deviceIDCRI_buf: B.lbuffer byte_pub (v deviceIDCRI_len) = B.alloca 0x00uy deviceIDCRI_len in
-(* hs9 *) let hs9 = HST.get () in
-
-   assume (B.(all_live hs9 [buf deviceID_pub;
-                            buf deviceIDCRI_buf]));
-   assume (B.(all_disjoint [loc_buffer deviceID_pub;
-                            loc_buffer deviceIDCRI_buf]));
-   printf "Creating DeviceID Certificate Signing Request Information\n" done;
-   create_deviceIDCRI
+  riot_core_step2
     (* version   *) deviceIDCSR_ingredients.deviceIDCSR_version
                     deviceIDCSR_ingredients.deviceIDCSR_s_common
                     deviceIDCSR_ingredients.deviceIDCSR_s_org
                     deviceIDCSR_ingredients.deviceIDCSR_s_country
     (* key usage *) deviceIDCSR_ingredients.deviceIDCSR_ku
     (* DeviceID  *) deviceID_pub
-    (*DeviceIDCRI*) deviceIDCRI_len
-                    deviceIDCRI_buf;
-(* hs10 *) let hs10 = HST.get () in
-
-  assume (B.(all_live hs10 [buf deviceID_priv;
-                            buf deviceIDCRI_buf;
-                            buf deviceIDCSR_buf]));
-  assume (B.(all_disjoint [loc_buffer deviceID_priv;
-                           loc_buffer deviceIDCRI_buf;
-                           loc_buffer deviceIDCSR_buf]));
-  printf "Signing and finalizing DeviceID Certificate Signing Request\n" done;
-  sign_and_finalize_deviceIDCSR
-    (*Signing Key*) deviceID_priv
-    (*DeviceIDCRI*) deviceIDCRI_len
-                    deviceIDCRI_buf
-    (*DeviceIDCSR*) deviceIDCSR_len
+                    deviceID_priv
+    (*DeviceIDCRI*) deviceIDCSR_len
                     deviceIDCSR_buf;
-(* hs11 *) let hs11 = HST.get () in
+  let _h_step2_post = HST.get () in
 
-(* Create AliasKeyTBS *)
-  let aliasKeyTBS_len: asn1_TLV_int32_of_type SEQUENCE = len_of_aliasKeyTBS
-                                                           aliasKeyCRT_ingredients.aliasKeyCrt_serialNumber
-                                                           aliasKeyCRT_ingredients.aliasKeyCrt_i_common
-                                                           aliasKeyCRT_ingredients.aliasKeyCrt_i_org
-                                                           aliasKeyCRT_ingredients.aliasKeyCrt_i_country
-                                                           aliasKeyCRT_ingredients.aliasKeyCrt_s_common
-                                                           aliasKeyCRT_ingredients.aliasKeyCrt_s_org
-                                                           aliasKeyCRT_ingredients.aliasKeyCrt_s_country
-                                                           aliasKeyCRT_ingredients.aliasKeyCrt_riot_version in
-  let aliasKeyTBS_buf: B.lbuffer byte_pub (v aliasKeyTBS_len) = B.alloca 0x00uy aliasKeyTBS_len in
+  (**) B.modifies_trans (
+    B.loc_buffer deviceID_pub  `B.loc_union`
+    B.loc_buffer deviceID_priv `B.loc_union`
+    B.loc_buffer aliasKey_pub  `B.loc_union`
+    B.loc_buffer aliasKey_priv `B.loc_union`
+    B.loc_buffer authKeyID
+  ) h0 _h_step2_pre (
+    B.loc_buffer deviceIDCSR_buf
+  ) _h_step2_post;
 
-(* hs12 *) let hs12 = HST.get () in
-  assume (B.(all_live hs12 [buf fwid;
-                            buf deviceID_pub;
-                            buf aliasKey_pub;
-                            buf aliasKeyCrt_keyID;
-                            buf aliasKeyTBS_buf]));
-  assume (B.(all_disjoint [loc_buffer fwid;
-                           loc_buffer deviceID_pub;
-                           loc_buffer aliasKey_pub;
-                           loc_buffer aliasKeyCrt_keyID;
-                           loc_buffer aliasKeyTBS_buf]));
+  assert (
+    deviceIDCSR_post
+      (cdi) (deviceID_label_len) (deviceID_label)
+      (deviceIDCSR_ingredients)
+      (deviceIDCSR_len) (deviceIDCSR_buf)
+      (h0) (_h_step2_post)
+  );
 
-  printf "Creating AliasKey Certificate TBS\n" done;
-  create_aliasKeyTBS
+  let _h_step3_pre = _h_step2_post in
+
+  (**) B.modifies_buffer_elim fwid (
+         B.loc_buffer deviceID_pub  `B.loc_union`
+         B.loc_buffer deviceID_priv `B.loc_union`
+         B.loc_buffer aliasKey_pub  `B.loc_union`
+         B.loc_buffer aliasKey_priv `B.loc_union`
+         B.loc_buffer authKeyID     `B.loc_union`
+         B.loc_buffer deviceIDCSR_buf
+  ) h0 _h_step3_pre;
+  (**) B.modifies_buffer_elim authKeyID     (B.loc_buffer deviceIDCSR_buf) _h_step1_post _h_step3_pre;
+  (**) B.modifies_buffer_elim deviceID_pub  (B.loc_buffer deviceIDCSR_buf) _h_step1_post _h_step3_pre;
+  (**) B.modifies_buffer_elim deviceID_priv (B.loc_buffer deviceIDCSR_buf) _h_step1_post _h_step3_pre;
+  (**) B.modifies_buffer_elim aliasKey_pub  (B.loc_buffer deviceIDCSR_buf) _h_step1_post _h_step3_pre;
+
+  riot_core_step3
     (aliasKeyCRT_ingredients.aliasKeyCrt_version)
     (aliasKeyCRT_ingredients.aliasKeyCrt_serialNumber)
     (aliasKeyCRT_ingredients.aliasKeyCrt_i_common)
@@ -781,345 +433,71 @@ let riot
     (aliasKeyCRT_ingredients.aliasKeyCrt_s_country)
     (fwid)
     (aliasKeyCRT_ingredients.aliasKeyCrt_ku)
-    (aliasKeyCrt_keyID)
+    (authKeyID)
     (aliasKeyCRT_ingredients.aliasKeyCrt_riot_version)
     (* DeviceID  *) deviceID_pub
+                    deviceID_priv
     (* AliasKey  *) aliasKey_pub
-    (*AliasKeyTBS*) aliasKeyTBS_len
-                    aliasKeyTBS_buf;
-
-(* hs13 *) let hs13 = HST.get () in
-  assume (B.(all_live hs13 [buf deviceID_priv;
-                            buf aliasKeyTBS_buf;
-                            buf aliasKeyCRT_buf]));
-  assume (B.(all_disjoint [loc_buffer deviceID_priv;
-                           loc_buffer aliasKeyTBS_buf;
-                           loc_buffer aliasKeyCRT_buf]));
-
-(* Sign AliasKeyTBS and Finalize AliasKeyCRT *)
-  printf "Signing and finalizing AliasKey Certificate\n" done;
-  sign_and_finalize_aliasKeyCRT
-    (*Signing Key*) deviceID_priv
-    (*AliasKeyTBS*) aliasKeyTBS_len
-                    aliasKeyTBS_buf
-    (*AliasKeyCRT*) aliasKeyCRT_len
+    (*AliasKeyTBS*) aliasKeyCRT_len
                     aliasKeyCRT_buf;
+  let _h_step3_post = HST.get () in
 
-(* hs14 *) let hs14 = HST.get () in
+  (**) B.modifies_trans (
+    B.loc_buffer deviceID_pub  `B.loc_union`
+    B.loc_buffer deviceID_priv `B.loc_union`
+    B.loc_buffer aliasKey_pub  `B.loc_union`
+    B.loc_buffer aliasKey_priv `B.loc_union`
+    B.loc_buffer authKeyID     `B.loc_union`
+    B.loc_buffer deviceIDCSR_buf
+  ) h0 _h_step3_pre (
+    B.loc_buffer aliasKeyCRT_buf
+  ) _h_step3_post;
+
+  (**) B.modifies_buffer_elim aliasKey_pub (
+         B.loc_buffer deviceIDCSR_buf `B.loc_union`
+         B.loc_buffer aliasKeyCRT_buf
+  ) _h_step1_post _h_step3_post;
+  assert (
+    aliasKeyCRT_post
+      (cdi) (fwid) (deviceID_label_len) (deviceID_label)
+      (aliasKeyCRT_ingredients)
+      (aliasKeyCRT_len) (aliasKeyCRT_buf)
+      (aliasKey_pub)
+      (h0) (_h_step3_post)
+  );
 
 (* hsf *) let hsf = HST.get () in
   HST.pop_frame ();
 (* hf *) let hf = HST.get () in
   (**) B.popped_modifies hsf hf;
+  (**) B.modifies_buffer_elim aliasKey_pub    (B.loc_region_only false (HS.get_tip hsf)) hsf hf;
+  (**) B.modifies_buffer_elim aliasKey_priv   (B.loc_region_only false (HS.get_tip hsf)) hsf hf;
+  (**) B.modifies_buffer_elim deviceIDCSR_buf (B.loc_region_only false (HS.get_tip hsf)) hsf hf;
+  (**) B.modifies_buffer_elim aliasKeyCRT_buf (B.loc_region_only false (HS.get_tip hsf)) hsf hf;
+  (**) B.modifies_fresh_frame_popped h0 hs0 (
+    B.loc_buffer aliasKey_pub    `B.loc_union`
+    B.loc_buffer aliasKey_priv   `B.loc_union`
+    B.loc_buffer deviceIDCSR_buf `B.loc_union`
+    B.loc_buffer aliasKeyCRT_buf
+  ) hsf hf;
 
-  lemma_help
-    byte_pub byte_sec
-    h0 hs0 hsf hf
-    cdi fwid deviceID_label aliasKey_label
-    aliasKey_pub aliasKey_priv deviceIDCSR_buf aliasKeyCRT_buf
-    hs1 hs2 hs3 hs4 hs5 hs6 hs7 hs8 hs9 hs10 hs11 hs12 hs13 hs14
-    32ul deviceID_pub 0x00uy
-    32ul deviceID_priv (u8 0x00)
-    32ul deviceID_pub_sec (u8 0x00)
-    20ul aliasKeyCrt_keyID 0x00uy
-    deviceIDCRI_len deviceIDCRI_buf 0x00uy
-    aliasKeyTBS_len aliasKeyTBS_buf 0x00uy;
-
-  assert ( B.as_seq hs5 cdi == B.as_seq h0 cdi /\
-           B.as_seq hs5 fwid == B.as_seq h0 fwid /\
-           B.as_seq hs5 aliasKey_label == B.as_seq h0 aliasKey_label);
-  assert ( aliasKey_post cdi fwid aliasKey_label_len aliasKey_label aliasKey_pub aliasKey_priv h0 hs6 );
-  assert ( B.as_seq hs6 aliasKey_pub  == B.as_seq hf aliasKey_pub /\
-           B.as_seq hs6 aliasKey_priv == B.as_seq hf aliasKey_priv );
-  assert ( aliasKey_post cdi fwid aliasKey_label_len aliasKey_label aliasKey_pub aliasKey_priv h0 hf );
-
-  assume (HST.equal_domains h0 hf)
-
-
-(*
-
-
-
-  // assert (HS.fresh_frame h0 hs0 /\ HS.get_tip hs0 == HS.get_tip hsf /\ HS.popped hsf hf);
-  // let _b1, _bv1, _bl1 = deviceID_pub, 0x00uy, 32ul in
-  // assert (B.alloc_post_mem_common _b1 hs0 hs1 (Seq.create (UInt32.v _bl1) _bv1) /\ B.frameOf _b1 == HS.get_tip hs0);
-  // let _b2, _bv2, _bl2 = deviceID_priv, (u8 0x00), 32ul in
-  // assert (B.alloc_post_mem_common _b2 hs1 hs2 (Seq.create (UInt32.v _bl2) _bv2) /\ B.frameOf _b2 == HS.get_tip hs1);
-  // let _b3, _bv3, _bl3 = deviceID_pub_sec, (u8 0x00), 32ul in
-  // assert (B.alloc_post_mem_common _b3 hs2 hs3 (Seq.create (UInt32.v _bl3) _bv3) /\ B.frameOf _b3 == HS.get_tip hs2);
-  // let _b4, _bv4, _bl4 = aliasKeyCrt_keyID, 0x00uy, 20ul in
-  // assert (B.alloc_post_mem_common _b4 hs3 hs4 (Seq.create (UInt32.v _bl4) _bv4) /\ B.frameOf _b4 == HS.get_tip hs3);
-  // assert (hs4 == hsf);
-  // let _b5, _bv5, _bl5 = deviceIDCRI_buf, 0x00uy, deviceIDCRI_len in
-  // assert (B.modifies (B.loc_buffer _b5) hs9 hs10); admit();
-
-  (**) let hs1 = HST.get () in
-  (**) B.modifies_trans B.loc_none h0 hs0 B.loc_none hs1;
-  // (**) B.modifies_buffer_elim cdi B.loc_none h0 hs1;
-  // (**) assume (B.(all_live hs1 [buf deviceID_pub;
-  //                               buf deviceID_priv;
-  //                               buf cdi;
-  //                               buf deviceID_label]));
-  // assume (B.(all_disjoint [loc_buffer deviceID_pub;
-  //                          loc_buffer deviceID_priv;
-  //                          loc_buffer cdi;
-  //                          loc_buffer deviceID_label]));
-
-  printf "Deriving DeviceID\n" done;
-  derive_DeviceID
-    (* pub *) deviceID_pub
-    (* priv*) deviceID_priv
-    (* cdi *) cdi
-    (* lbl *) deviceID_label_len
-              deviceID_label;
-
-  (**) let hsd = HST.get () in
-  (**) B.modifies_trans
-          B.loc_none h0 hs1
-         (B.loc_buffer deviceID_pub `B.loc_union` B.loc_buffer deviceID_priv) hsd;
-  // (**) B.modifies_buffer_elim cdi (B.loc_buffer deviceID_pub `B.loc_union` B.loc_buffer deviceID_priv) h0 hsd;
-
-  printf "Deriving AliasKey\n" done;
-  derive_AliasKey
-    (* pub *) aliasKey_pub
-    (* priv*) aliasKey_priv
-    (* cdi *) cdi
-    (* fwid*) fwid
-    (* lbl *) aliasKey_label_len
-              aliasKey_label;
-
-  (**) let hsa = HST.get () in
-  (**) B.modifies_trans
-         (B.loc_buffer deviceID_pub `B.loc_union ` B.loc_buffer deviceID_priv) h0 hsd
-         (B.loc_buffer aliasKey_pub `B.loc_union` B.loc_buffer aliasKey_priv) hsa;
-
-  classify_public_buffer 32ul deviceID_pub deviceID_pub_sec;
-
-  // assert ((B.loc_buffer deviceID_pub `B.loc_union` B.loc_buffer deviceID_priv) `B.loc_union`
-  //                     (B.loc_buffer aliasKey_pub `B.loc_union` B.loc_buffer aliasKey_priv)
-  //         ==
-  //         B.loc_buffer deviceID_pub `B.loc_union` B.loc_buffer deviceID_priv `B.loc_union`
-  //                     B.loc_buffer aliasKey_pub `B.loc_union` B.loc_buffer aliasKey_priv); admit()
-
-  (**) let hsa1 = HST.get () in
-  assert (B.modifies ((B.loc_buffer deviceID_pub `B.loc_union` B.loc_buffer deviceID_priv) `B.loc_union`
-                      (B.loc_buffer aliasKey_pub `B.loc_union` B.loc_buffer aliasKey_priv)) h0 hsa); admit();
-  // (**) B.modifies_trans
-  //        (B.loc_buffer deviceID_pub `B.loc_union` B.loc_buffer deviceID_priv `B.loc_union`
-  //         B.loc_buffer aliasKey_pub `B.loc_union` B.loc_buffer aliasKey_priv) h0 hsa
-  //        (B.loc_buffer deviceID_pub_sec) hsa1;
-  derive_authKeyID
-    aliasKeyCrt_keyID
-    deviceID_pub_sec;
-
-
-  (**) let hsf = HST.get () in
-  // assert (B.modifies (B.loc_buffer deviceID_pub `B.loc_union` B.loc_buffer deviceID_priv) hs0 hsf);
-  HST.pop_frame ();
-  (**) let hf = HST.get () in
-  (**) B.popped_modifies hsf hf;
-  assume (B.modifies (B.loc_all_regions_from false (HS.get_tip hs0) `B.loc_union`
-                      (B.loc_buffer aliasKey_pub `B.loc_union` B.loc_buffer aliasKey_priv)) hs0 hsf);
-  B.modifies_fresh_frame_popped h0 hs0 (B.loc_buffer aliasKey_pub `B.loc_union` B.loc_buffer aliasKey_priv) hsf hf;
-  // assert (B.modifies (B.loc_buffer deviceID_pub `B.loc_union` B.loc_buffer deviceID_priv) hs0 hf);
-  // (**) B.modifies_remove_fresh_frame h0 hs0 hf B.loc_none;
-  (**) assert (B.modifies (B.loc_buffer aliasKey_pub `B.loc_union` B.loc_buffer aliasKey_priv) h0 hf);
-  (**) assume (HST.equal_domains h0 hf)
-
-(*)
-  B.modifies_fresh_frame_popped h0 hs0 B.loc_none hs0 hf;
-  Set.lemma_equal_intro (Map.domain (HS.get_hmap h0)) (Map.domain (HS.get_hmap hf));
-  assert (Set.equal (Map.domain (HS.get_hmap h0)) (Map.domain (HS.get_hmap hf)));
-  // HST.lemma_same_refs_in_all_regions_intro h0 hf;
-  // assert (HST.same_refs_in_all_regions h0 hf);
   assert (HST.equal_domains h0 hf);
-  admit();
 
-(* Derive DeviceID *)
-  let deviceID_pub : B.lbuffer byte_pub 32 = B.alloca 0x00uy    32ul in
-  let deviceID_priv: B.lbuffer byte_sec 32 = B.alloca (u8 0x00) 32ul in
+  assert (aliasKey_post cdi fwid aliasKey_label_len aliasKey_label aliasKey_pub aliasKey_priv h0 hf);
 
-  let h = HST.get () in
-  // assume (B.(all_live h [buf deviceID_pub;
-  //                        buf deviceID_priv;
-  //                        buf cdi;
-  //                        buf deviceID_label]));
-  // assume (B.(all_disjoint [loc_buffer deviceID_pub;
-  //                          loc_buffer deviceID_priv;
-  //                          loc_buffer cdi;
-  //                          loc_buffer deviceID_label]));
-  printf "Deriving DeviceID\n" done;
-  derive_DeviceID
-    (* pub *) deviceID_pub
-    (* priv*) deviceID_priv
-    (* cdi *) cdi
-    (* lbl *) deviceID_label_len
-              deviceID_label;
-  HST.pop_frame ();
-  // let hf = HST.get () in
-  // assume (HST.equal_domains h0 hf)
+  assert (
+    deviceIDCSR_post
+      (cdi) (deviceID_label_len) (deviceID_label)
+      (deviceIDCSR_ingredients)
+      (deviceIDCSR_len) (deviceIDCSR_buf)
+      (h0) (hf)
+  );
 
-(* A workaround to derive authKeyID for now *)
-  let deviceID_pub_sec: B.lbuffer byte_sec 32 = B.alloca (u8 0x00) 32ul in
-  let aliasKeyCrt_keyID: B.lbuffer byte_pub 20 = B.alloca 0x00uy 20ul in
-  classify_public_buffer 32ul deviceID_pub deviceID_pub_sec;
-  derive_authKeyID
-    aliasKeyCrt_keyID
-    deviceID_pub_sec;
-  // let aliasKeyCrt_keyID: datatype_of_asn1_type OCTET_STRING = (|20ul, B32.of_buffer 20ul aliasKeyCrt_keyID_buf|) in
-
-(* Derive AliasKey *)
-  printf "Deriving AliasKey\n" done;
-  derive_AliasKey
-    (* pub *) aliasKey_pub
-    (* priv*) aliasKey_priv
-    (* cdi *) cdi
-    (* fwid*) fwid
-    (* lbl *) aliasKey_label_len
-              aliasKey_label;
-
-  // let h_AliasKey = HST.get () in
-
-  let h2 = HST.get () in
-  // assume (HS.poppable h);
-  HST.pop_frame();
-
-  // B.modifies_fresh_frame_popped
-
-  let h3 = HST.get () in
-  assume (B.modifies B.loc_none h2 h3);
-  // assume (HST.equal_domains h0 h3);
-
-
-(* Create DeviceIDCRI *)
-   let deviceIDCRI_len: asn1_TLV_int32_of_type SEQUENCE = len_of_deviceIDCRI
-                                                            deviceIDCSR_ingredients.deviceIDCSR_version
-                                                            deviceIDCSR_ingredients.deviceIDCSR_s_common
-                                                            deviceIDCSR_ingredients.deviceIDCSR_s_org
-                                                            deviceIDCSR_ingredients.deviceIDCSR_s_country in
-   let deviceIDCRI_buf: B.lbuffer byte_pub (v deviceIDCRI_len) = B.alloca 0x00uy deviceIDCRI_len in
-
-   let h = HST.get () in
-   assume (B.(all_live h [buf deviceID_pub;
-                          buf deviceIDCRI_buf]));
-   assume (B.(all_disjoint [loc_buffer deviceID_pub;
-                            loc_buffer deviceIDCRI_buf]));
-
-   printf "Creating DeviceID Certificate Signing Request Information\n" done;
-   create_deviceIDCRI
-    (* version   *) deviceIDCSR_ingredients.deviceIDCSR_version
-                    deviceIDCSR_ingredients.deviceIDCSR_s_common
-                    deviceIDCSR_ingredients.deviceIDCSR_s_org
-                    deviceIDCSR_ingredients.deviceIDCSR_s_country
-    (* key usage *) deviceIDCSR_ingredients.deviceIDCSR_ku
-    (* DeviceID  *) deviceID_pub
-    (*DeviceIDCRI*) deviceIDCRI_len
-                    deviceIDCRI_buf;
-
-(* Zhe 10/06: Hard to be proved even with 100 more z3rlimits. *)
-  let h = HST.get () in
-  assume (B.(all_live h [buf deviceID_priv;
-                         buf deviceIDCRI_buf;
-                         buf deviceIDCSR_buf]));
-  assume (B.(all_disjoint [loc_buffer deviceID_priv;
-                           loc_buffer deviceIDCRI_buf;
-                           loc_buffer deviceIDCSR_buf]));
-
-  // assume (0 < v deviceIDCRI_len);
-  // assume (valid_deviceIDCSR_ingredients deviceIDCSR_len);
-  // assume (v deviceIDCSR_len == length_of_deviceIDCSR deviceIDCRI_len);
-
-(* Sign AliasKeyTBS and Finalize AliasKeyCRT *)
-  printf "Signing and finalizing DeviceID Certificate Signing Request\n" done;
-  sign_and_finalize_deviceIDCSR
-    (*Signing Key*) deviceID_priv
-    (*DeviceIDCRI*) deviceIDCRI_len
-                    deviceIDCRI_buf
-    (*DeviceIDCSR*) deviceIDCSR_len
-                    deviceIDCSR_buf;
-(* Create AliasKeyTBS *)
-  let aliasKeyTBS_len: asn1_TLV_int32_of_type SEQUENCE = len_of_aliasKeyTBS
-                                                           aliasKeyCRT_ingredients.aliasKeyCrt_serialNumber
-                                                           aliasKeyCRT_ingredients.aliasKeyCrt_i_common
-                                                           aliasKeyCRT_ingredients.aliasKeyCrt_i_org
-                                                           aliasKeyCRT_ingredients.aliasKeyCrt_i_country
-                                                           aliasKeyCRT_ingredients.aliasKeyCrt_s_common
-                                                           aliasKeyCRT_ingredients.aliasKeyCrt_s_org
-                                                           aliasKeyCRT_ingredients.aliasKeyCrt_s_country
-                                                           aliasKeyCRT_ingredients.aliasKeyCrt_riot_version in
-  let aliasKeyTBS_buf: B.lbuffer byte_pub (v aliasKeyTBS_len) = B.alloca 0x00uy aliasKeyTBS_len in
-
-  let h = HST.get () in
-  assume (B.(all_live h [buf fwid;
-                         buf deviceID_pub;
-                         buf aliasKey_pub;
-                         buf aliasKeyCrt_keyID;
-                         buf aliasKeyTBS_buf]));
-
-  assume (B.(all_disjoint [loc_buffer fwid;
-                           loc_buffer deviceID_pub;
-                           loc_buffer aliasKey_pub;
-                           loc_buffer aliasKeyCrt_keyID;
-                           loc_buffer aliasKeyTBS_buf]));
-
-  printf "Creating AliasKey Certificate TBS\n" done;
-  create_aliasKeyTBS
-    (aliasKeyCRT_ingredients.aliasKeyCrt_version)
-    (aliasKeyCRT_ingredients.aliasKeyCrt_serialNumber)
-    (aliasKeyCRT_ingredients.aliasKeyCrt_i_common)
-    (aliasKeyCRT_ingredients.aliasKeyCrt_i_org)
-    (aliasKeyCRT_ingredients.aliasKeyCrt_i_country)
-    (aliasKeyCRT_ingredients.aliasKeyCrt_notBefore)
-    (aliasKeyCRT_ingredients.aliasKeyCrt_notAfter)
-    (aliasKeyCRT_ingredients.aliasKeyCrt_s_common)
-    (aliasKeyCRT_ingredients.aliasKeyCrt_s_org)
-    (aliasKeyCRT_ingredients.aliasKeyCrt_s_country)
-    (fwid)
-    (aliasKeyCRT_ingredients.aliasKeyCrt_ku)
-    (aliasKeyCrt_keyID)
-    (aliasKeyCRT_ingredients.aliasKeyCrt_riot_version)
-    (* DeviceID  *) deviceID_pub
-    (* AliasKey  *) aliasKey_pub
-    (*AliasKeyTBS*) aliasKeyTBS_len
-                    aliasKeyTBS_buf;
-
-  assume (B.(all_live h [buf deviceID_priv;
-                         buf aliasKeyTBS_buf;
-                         buf aliasKeyCRT_buf]));
-  assume (B.(all_disjoint [loc_buffer deviceID_priv;
-                           loc_buffer aliasKeyTBS_buf;
-                           loc_buffer aliasKeyCRT_buf]));
-
-(* Sign AliasKeyTBS and Finalize AliasKeyCRT *)
-  printf "Signing and finalizing AliasKey Certificate\n" done;
-  sign_and_finalize_aliasKeyCRT
-    (*Signing Key*) deviceID_priv
-    (*AliasKeyTBS*) aliasKeyTBS_len
-                    aliasKeyTBS_buf
-    (*AliasKeyCRT*) aliasKeyCRT_len
-                    aliasKeyCRT_buf;
-
-  let h = HST.get () in
-  assume (HS.poppable h);
-  HST.pop_frame();
-
-  let h = HST.get () in
-  assume (HST.equal_domains h0 h);
-  assume (B.(modifies (loc_buffer deviceIDCSR_buf `loc_union`
-                       loc_buffer aliasKeyCRT_buf `loc_union`
-                       loc_buffer aliasKey_pub    `loc_union`
-                       loc_buffer aliasKey_priv ) h0 h) );
-  assume (B.as_seq h_AliasKey aliasKey_pub  == B.as_seq h aliasKey_pub /\
-          B.as_seq h_AliasKey aliasKey_priv == B.as_seq h aliasKey_priv);
-  // assume (aliasKey_post cdi fwid aliasKey_label_len aliasKey_label aliasKey_pub aliasKey_priv h0 h)
-  // assume (riot_post
-  //                       (cdi)
-  //                       (fwid)
-  //                       (deviceID_label_len) (deviceID_label)
-  //                       (aliasKey_label_len) (aliasKey_label)
-  //                       (deviceIDCSR_ingredients)
-  //                       (aliasKeyCRT_ingredients)
-  //                       (aliasKey_pub) (aliasKey_priv)
-  //                       (deviceIDCSR_len) (deviceIDCSR_buf)
-  //                       (aliasKeyCRT_len) (aliasKeyCRT_buf)
-  //                       (h0) (h))
+  assert (
+    aliasKeyCRT_post
+      (cdi) (fwid) (deviceID_label_len) (deviceID_label)
+      (aliasKeyCRT_ingredients)
+      (aliasKeyCRT_len) (aliasKeyCRT_buf)
+      (aliasKey_pub)
+      (h0) (hf)
+  )
