src/riot/RIoT.Impl.Crypto.fst
@@ -1,5 +1,7 @@
 module RIoT.Impl.Crypto
 
+open LowStar.Comment
+open LowStar.Printf
 module Fail = LowStar.Failure
 module B = LowStar.Buffer
 module IB = LowStar.ImmutableBuffer
@@ -191,3 +193,280 @@ let derive_authKeyID
   declassify_secret_buffer 20ul authKeyID_sec authKeyID;
 
   HST.pop_frame ()
+
+[@@ "opaque_to_smt"]
+unfold
+let riot_core_step1_pre
+  (h: HS.mem)
+(* Inputs *)
+  (cdi : B.lbuffer byte_sec 32)
+  (fwid: B.lbuffer byte_sec 32)
+  (deviceID_label_len: size_t)
+  (deviceID_label: B.lbuffer byte_sec (v deviceID_label_len))
+  (aliasKey_label_len: size_t)
+  (aliasKey_label: B.lbuffer byte_sec (v aliasKey_label_len))
+(* Outputs *)
+  (deviceID_pub : B.lbuffer byte_pub 32)
+  (deviceID_priv: B.lbuffer byte_sec 32)
+  (aliasKey_pub : B.lbuffer byte_pub 32)
+  (aliasKey_priv: B.lbuffer byte_sec 32)
+  (authKeyID    : B.lbuffer byte_pub 20)
+= B.(all_live h [buf cdi;
+                 buf fwid;
+                 buf deviceID_label;
+                 buf aliasKey_label;
+                 buf deviceID_pub;
+                 buf deviceID_priv;
+                 buf aliasKey_pub;
+                 buf aliasKey_priv;
+                 buf authKeyID]) /\
+  B.(all_disjoint [loc_buffer cdi;
+                   loc_buffer fwid;
+                   loc_buffer deviceID_label;
+                   loc_buffer aliasKey_label;
+                   loc_buffer deviceID_pub;
+                   loc_buffer deviceID_priv;
+                   loc_buffer aliasKey_pub;
+                   loc_buffer aliasKey_priv;
+                   loc_buffer authKeyID]) /\
+  valid_hkdf_lbl_len deviceID_label_len /\
+  valid_hkdf_lbl_len aliasKey_label_len
+
+[@@ "opaque_to_smt"]
+unfold
+let riot_core_step1_post
+  (h0: HS.mem) (h1: HS.mem)
+(* Inputs *)
+  (cdi : B.lbuffer byte_sec 32)
+  (fwid: B.lbuffer byte_sec 32)
+  (deviceID_label_len: size_t)
+  (deviceID_label: B.lbuffer byte_sec (v deviceID_label_len))
+  (aliasKey_label_len: size_t)
+  (aliasKey_label: B.lbuffer byte_sec (v aliasKey_label_len))
+(* Outputs *)
+  (deviceID_pub : B.lbuffer byte_pub 32)
+  (deviceID_priv: B.lbuffer byte_sec 32)
+  (aliasKey_pub : B.lbuffer byte_pub 32)
+  (aliasKey_priv: B.lbuffer byte_sec 32)
+  (authKeyID    : B.lbuffer byte_pub 20
+              { riot_core_step1_pre (h0)
+                     (cdi) (fwid)
+                     (deviceID_label_len) (deviceID_label)
+                     (aliasKey_label_len) (aliasKey_label)
+                     (deviceID_pub) (deviceID_priv)
+                     (aliasKey_pub) (aliasKey_priv)
+                     (authKeyID) })
+=
+  // let deviceID_pub_seq, deviceID_priv_seq = derive_DeviceID_spec
+  //                                             (B.as_seq h0 cdi)
+  //                                             (deviceID_label_len)
+  //                                             (B.as_seq h0 deviceID_label) in
+  // let deviceID_pub_sec_seq = classify_public_bytes (B.as_seq h1 deviceID_pub) in
+  (B.modifies (B.loc_buffer deviceID_pub  `B.loc_union`
+               B.loc_buffer deviceID_priv `B.loc_union`
+               B.loc_buffer aliasKey_pub  `B.loc_union`
+               B.loc_buffer aliasKey_priv `B.loc_union`
+               B.loc_buffer authKeyID) h0 h1) /\
+  ((B.as_seq h1 deviceID_pub  <: lbytes_pub 32),
+   (B.as_seq h1 deviceID_priv <: lbytes_sec 32)) == derive_DeviceID_spec
+                                                      (B.as_seq h0 cdi)
+                                                      (deviceID_label_len)
+                                                      (B.as_seq h0 deviceID_label) /\
+  ((B.as_seq h1 aliasKey_pub  <: lbytes_pub 32),
+   (B.as_seq h1 aliasKey_priv <: lbytes_sec 32)) == derive_AliasKey_spec
+                                                       (B.as_seq h0 cdi)
+                                                       (B.as_seq h0 fwid)
+                                                       (aliasKey_label_len)
+                                                       (B.as_seq h0 aliasKey_label) /\
+  (B.as_seq h1 authKeyID == derive_authKeyID_spec (classify_public_bytes (B.as_seq h1 deviceID_pub)))
+
+#set-options "--z3rlimit 20 --fuel 0 --ifuel 0 --using_facts_from '* -FStar.Tactics -FStar.Reflection'"
+[@@ "opaque_to_smt"]
+let riot_core_step1
+(* Inputs *)
+  (cdi : B.lbuffer byte_sec 32)
+  (fwid: B.lbuffer byte_sec 32)
+  (deviceID_label_len: size_t)
+  (deviceID_label: B.lbuffer byte_sec (v deviceID_label_len))
+  (aliasKey_label_len: size_t)
+  (aliasKey_label: B.lbuffer byte_sec (v aliasKey_label_len))
+(* Outputs *)
+  (deviceID_pub : B.lbuffer byte_pub 32)
+  (deviceID_priv: B.lbuffer byte_sec 32)
+  (aliasKey_pub : B.lbuffer byte_pub 32)
+  (aliasKey_priv: B.lbuffer byte_sec 32)
+  (authKeyID    : B.lbuffer byte_pub 20)
+: HST.Stack unit
+  (requires fun h -> riot_core_step1_pre (h)
+                     (cdi) (fwid)
+                     (deviceID_label_len) (deviceID_label)
+                     (aliasKey_label_len) (aliasKey_label)
+                     (deviceID_pub) (deviceID_priv)
+                     (aliasKey_pub) (aliasKey_priv)
+                     (authKeyID))
+  (ensures fun h0 _ h1 -> riot_core_step1_post (h0) (h1)
+                     (cdi) (fwid)
+                     (deviceID_label_len) (deviceID_label)
+                     (aliasKey_label_len) (aliasKey_label)
+                     (deviceID_pub) (deviceID_priv)
+                     (aliasKey_pub) (aliasKey_priv)
+                     (authKeyID))
+= (**) let h0 = HST.get () in
+  HST.push_frame ();
+  (**) let hs0 = HST.get () in
+  (**) B.fresh_frame_modifies h0 hs0;
+
+(* Derive DeviceID *)
+  // let deviceID_pub : B.lbuffer byte_pub 32 = B.alloca 0x00uy    32ul in
+  // let deviceID_priv: B.lbuffer byte_sec 32 = B.alloca (u8 0x00) 32ul in
+  let deviceID_pub_sec: B.lbuffer byte_sec 32 = B.alloca (u8 0x00) 32ul in
+  printf "Deriving DeviceID\n" done;
+  derive_DeviceID
+    (* pub *) deviceID_pub
+    (* priv*) deviceID_priv
+    (* cdi *) cdi
+    (* lbl *) deviceID_label_len
+              deviceID_label;
+
+  printf "Deriving AliasKey\n" done;
+  derive_AliasKey
+    (* pub *) aliasKey_pub
+    (* priv*) aliasKey_priv
+    (* cdi *) cdi
+    (* fwid*) fwid
+    (* lbl *) aliasKey_label_len
+              aliasKey_label;
+
+  classify_public_buffer 32ul deviceID_pub deviceID_pub_sec;
+
+  derive_authKeyID
+    authKeyID
+    deviceID_pub_sec;
+
+  (**) let hsf = HST.get () in
+  HST.pop_frame ();
+  (**) let hf = HST.get () in
+  (**) B.popped_modifies hsf hf;
+  // assume (HST.equal_domains h0 hf);
+  // assume (B.modifies (
+               // B.loc_buffer deviceID_pub  `B.loc_union`
+               // B.loc_buffer deviceID_priv `B.loc_union`
+               // B.loc_buffer aliasKey_pub  `B.loc_union`
+               // B.loc_buffer aliasKey_priv `B.loc_union`
+               // B.loc_buffer authKeyID) h0 hf);
+()
+
+(*)
+#reset-options
+#set-options "--z3rlimit 256 --fuel 0 --ifuel 0 --using_facts_from '* -FStar.Tactics -FStar.Reflection'"
+[@@ "opaque_to_smt"]
+let riot_core_step1
+(* Inputs *)
+  (cdi : B.lbuffer byte_sec 32)
+  (fwid: B.lbuffer byte_sec 32)
+  (deviceID_label_len: size_t)
+  (deviceID_label: B.lbuffer byte_sec (v deviceID_label_len))
+  (aliasKey_label_len: size_t)
+  (aliasKey_label: B.lbuffer byte_sec (v aliasKey_label_len))
+(* Outputs *)
+  (aliasKey_pub: B.lbuffer byte_pub 32)
+  (aliasKey_priv: B.lbuffer uint8 32)
+  (authKeyID: B.lbuffer byte_pub 20)
+: HST.Stack unit
+  (requires fun h -> riot_core_step1_pre (h)
+                     (cdi) (fwid)
+                     (deviceID_label_len) (deviceID_label)
+                     (aliasKey_label_len) (aliasKey_label)
+                     (aliasKey_pub) (aliasKey_priv)
+                     (authKeyID))
+  (ensures fun h0 _ h1 -> riot_core_step1_post (h0) (h1)
+                     (cdi) (fwid)
+                     (deviceID_label_len) (deviceID_label)
+                     (aliasKey_label_len) (aliasKey_label)
+                     (aliasKey_pub) (aliasKey_priv)
+                     (authKeyID))
+= (**) let h0 = HST.get () in
+  HST.push_frame ();
+  (**) let hs0 = HST.get () in
+  (**) B.fresh_frame_modifies h0 hs0;
+
+(* Derive DeviceID *)
+  let deviceID_pub : B.lbuffer byte_pub 32 = B.alloca 0x00uy    32ul in
+  let hs1 = HST.get () in
+  let deviceID_priv: B.lbuffer byte_sec 32 = B.alloca (u8 0x00) 32ul in
+  let hs2 = HST.get () in
+  let deviceID_pub_sec: B.lbuffer byte_sec 32 = B.alloca (u8 0x00) 32ul in
+  let hs3 = HST.get () in
+  let hs4 = HST.get () in
+
+  assume (
+    B.(all_live hs4 [buf deviceID_pub;
+                     buf deviceID_priv;
+                     buf cdi;
+                     buf deviceID_label]) /\
+    B.(all_disjoint [loc_buffer deviceID_pub;
+                     loc_buffer deviceID_priv;
+                     loc_buffer cdi;
+                     loc_buffer deviceID_label])
+  );
+  printf "Deriving DeviceID\n" done;
+  derive_DeviceID
+    (* pub *) deviceID_pub
+    (* priv*) deviceID_priv
+    (* cdi *) cdi
+    (* lbl *) deviceID_label_len
+              deviceID_label;
+(* hs5 *) let hs5 = HST.get () in
+
+  assume (
+    B.(all_live hs5 [buf aliasKey_pub;
+                     buf aliasKey_priv;
+                     buf cdi;
+                     buf fwid;
+                     buf aliasKey_label]) /\
+    B.(all_disjoint [loc_buffer aliasKey_pub;
+                     loc_buffer aliasKey_priv;
+                     loc_buffer cdi;
+                     loc_buffer fwid;
+                     loc_buffer aliasKey_label])
+  );
+  printf "Deriving AliasKey\n" done;
+  derive_AliasKey
+    (* pub *) aliasKey_pub
+    (* priv*) aliasKey_priv
+    (* cdi *) cdi
+    (* fwid*) fwid
+    (* lbl *) aliasKey_label_len
+              aliasKey_label;
+(* hs6 *) let hs6 = HST.get () in
+
+  assume (
+    B.live hs6 deviceID_pub /\ B.live hs6 deviceID_pub_sec /\
+    B.disjoint deviceID_pub deviceID_pub_sec
+  );
+  classify_public_buffer 32ul deviceID_pub deviceID_pub_sec;
+(* hs7 *) let hs7 = HST.get () in
+
+  assume (
+    B.live hs7 authKeyID /\ B.live hs7 deviceID_pub_sec /\
+    B.disjoint authKeyID deviceID_pub_sec
+  );
+  derive_authKeyID
+    authKeyID
+    deviceID_pub_sec;
+(* hs8 *) let hs8 = HST.get () in
+
+(* hsf *) let hsf = HST.get () in
+  HST.pop_frame ();
+(* hf *) let hf = HST.get () in
+  (**) B.popped_modifies hsf hf;
+  assume (HST.equal_domains h0 hf);
+  assume ((B.modifies (B.loc_buffer aliasKey_pub  `B.loc_union`
+                       B.loc_buffer aliasKey_priv `B.loc_union`
+                       B.loc_buffer authKeyID) h0 hf));
+  assume (((B.as_seq hf aliasKey_pub  <: lbytes_pub 32),
+           (B.as_seq hf aliasKey_priv <: lbytes_sec 32)) == derive_AliasKey_spec
+                                                       (B.as_seq h0 cdi)
+                                                       (B.as_seq h0 fwid)
+                                                       (aliasKey_label_len)
+                                                       (B.as_seq h0 aliasKey_label))
